bind works

pulse/lib/steel/pulse/Pulse.Prover.Common.fsti
@@ -9,82 +9,255 @@ open Pulse.Typing.Metatheory
 open Pulse.Checker.VPropEquiv
 open Pulse.Prover.Util
 
+open Pulse.Checker.Auto.Elims
+
 module T = FStar.Tactics
 
 module Psubst = Pulse.Prover.Substs
 
 let vprop_typing (g:env) (t:term) = tot_typing g t tm_vprop
 
-noeq
-type preamble = {
+noeq type preamble = {
   g0 : env;
-
+  
   ctxt : vprop;
   ctxt_typing : vprop_typing g0 ctxt;
 
-  t : st_term;
-  c : comp_st;
-
-  uvs : uvs:env { disjoint uvs g0 }
+  goals : vprop;
 }
 
-let pst_env (#g0:env) (uvs:env { disjoint uvs g0 }) (ss:Psubst.t g0) =
-  push_env g0 (psubst_env (filter_ss uvs ss) ss)
+type ss_t = Map.t var term
 
-noeq
-type prover_state (preamble:preamble) = {
-  ss : ss:Psubst.t preamble.g0 {
-    well_typed_ss preamble.uvs ss
-  };
+val as_subst (ss:ss_t) : subst
 
-  solved_goals : term;
+let shift (ss:ss_t) = shift_subst (as_subst ss)
 
-  unsolved_goals : list term;
+let op_Array_Access (ss:ss_t) (t:term) =
+  subst_term t (as_subst ss)
 
-  remaining_ctxt : list term;
+let op_String_Access = Map.sel
 
-  steps : st_term;
+let op_Star = tm_star
 
-  t_typing
-    : st_typing (pst_env preamble.uvs ss)
-                (Psubst.subst_st_term ss preamble.t)
-                (Psubst.subst_comp ss preamble.c);
+let well_typed_ss (ss:ss_t) (uvs g:env) =
+  forall (x:var).
+  Map.contains ss x ==> (Set.mem x (dom uvs) /\
+                         tot_typing g ss.[x] (ss.(Some?.v (lookup uvs x))))
 
-  unsolved_goals_typing
-    : vprop_typing (pst_env preamble.uvs ss)
-                   (list_as_vprop unsolved_goals);
+noeq type prover_state (preamble:preamble) = {
+  g : g:env { g `env_extends` preamble.g0 };
 
-  remaining_ctxt_typing
-    : vprop_typing preamble.g0 (list_as_vprop remaining_ctxt);
+  remaining_ctxt : list vprop;
+
+  uvs : uvs:env { disjoint uvs g };
+  ss : ss:ss_t { well_typed_ss ss uvs g};
+
+  solved : vprop;
+  unsolved : list vprop;
+
+  k : continuation_elaborator preamble.g0 preamble.ctxt
+                              g (list_as_vprop remaining_ctxt * ss.(solved));
+
+  goals_inv : vprop_equiv g preamble.goals (list_as_vprop unsolved * solved);
+}
+
+let covers (ss:ss_t) (uvs:env) =
+  Set.equal (Map.domain ss) (dom uvs)
+
+let is_terminal (#preamble:_) (st:prover_state preamble) =
+  st.unsolved == [] /\ covers st.ss st.uvs
+
+
+val prove
+  (#g:env) (#ctxt:vprop) (ctxt_typing:vprop_typing g ctxt)
+  (uvs:env { disjoint g uvs })
+  (#goals:vprop) (goals_typing:vprop_typing (push_env g uvs) goals)
+
+  : T.Tac (g1 : env { g1 `env_extends` g /\ disjoint g1 uvs } &
+           ss : ss_t { well_typed_ss ss uvs g1 } &
+           remaining_ctxt : vprop &
+           k : continuation_elaborator g ctxt g1 (ss.(goals) * remaining_ctxt))
+
+open Pulse.Checker.Common
+
+val check_stapp_no_ctxt (g:env) (t:st_term { Tm_STApp? t.term })
+  : T.Tac (uvs : env { disjoint uvs g } &
+           t:st_term &
+           c:comp_st &
+           st_typing (push_env g uvs) t c)
+
+let extend_post_hint_opt_g (g:env) (post_hint:post_hint_opt g) (g1:env { g1 `env_extends` g })
+  : p:post_hint_opt g1 { p == post_hint } =
+  match post_hint with
+  | None -> None
+  | Some post_hint ->
+    assert (g `env_extends` post_hint.g);
+    assert (g1 `env_extends` g);
+    assert (g1 `env_extends` post_hint.g);
+    Some post_hint
+
+val add_frame (#g:env) (#t:st_term) (#c:comp_st) (t_typing:st_typing g t c)
+  (frame:vprop)
+  : T.Tac (t':st_term &
+           c':comp_st { c' == add_frame c frame } &
+           st_typing g t' c')
+
+val st_typing_subst (g:env) (uvs:env { disjoint uvs g }) (t:st_term) (c:comp_st)
+  (_:st_typing (push_env g uvs) t c)
+  (ss:ss_t { well_typed_ss ss uvs g })
+  : T.Tac (st_typing g (subst_st_term t (as_subst ss)) (subst_comp c (as_subst ss)))
+
+val st_typing_weakening
+  (g:env) (g':env { disjoint g g' })
+  (t:st_term) (c:comp_st) (_:st_typing (push_env g g') t c)
+  (g1:env { g1 `env_extends` g /\ disjoint g1 g' })
+  : T.Tac (st_typing (push_env g1 g') t c)
+
+// This is implemented in Pulse.Checker.Bind
+val  mk_bind' (g:env)
+              (pre:term)
+              (e1:st_term)
+              (e2:st_term)
+              (c1:comp_st)
+              (c2:comp_st)
+              (px:nvar { ~ (Set.mem (snd px) (dom g)) })
+              (d_e1:st_typing g e1 c1)
+              (d_c1res:tot_typing g (comp_res c1) (tm_type (comp_u c1)))
+              (d_e2:st_typing (push_binding g (snd px) (fst px) (comp_res c1)) (open_st_term_nv e2 px) c2)
+              (post_hint:post_hint_opt g { comp_post_matches_hint c2 post_hint })
+              (_:squash (
+                 let _, x = px in
+                 comp_pre c1 == pre /\
+                 None? (lookup g x) /\
+                 (~(x `Set.mem` freevars_st e2)) /\
+                 open_term (comp_post c1) x == comp_pre c2))
+  : T.Tac (checker_result_t g pre post_hint)
+
+#push-options "--z3rlimit_factor 8 --fuel 1 --ifuel 1 --admit_smt_queries true"
+let check_bind
+  (g:env)
+  (t:st_term {Tm_Bind? t.term})
+  (pre:term)
+  (pre_typing:tot_typing g pre tm_vprop)
+  (post_hint:post_hint_opt g)
+  (check:check_t)
+  : T.Tac (checker_result_t g pre post_hint) =
+
+  let Tm_Bind { binder=b; head=e1; body=e2 } = t.term in
+
+  match e1.term with
+  | Tm_STApp _ ->
+    let (| uvs1, e1, c1, d1 |) = check_stapp_no_ctxt g e1 in
+    let c10 = c1 in
+    // magic is comp_pre c1 typing, get from inversion of d1 
+    let (| g1, ss1, remaining_pre, k |) =
+      prove pre_typing uvs1 #(comp_pre c1) (magic ()) in
+    let x = fresh g1 in
+    let px = b.binder_ppname, x in
+    // TODO: if the binder is annotated, check subtyping
+    let g2 = push_binding g1 x b.binder_ppname ss1.(comp_res c1) in
+    let pre_e2 = open_term_nv (subst_term (comp_post c1) (shift ss1)) px * remaining_pre in
+    assert (g2 `env_extends` g1);
+    // magic is the typing of pre_e2 in g2
+    // remaining_pre is well-typed, may be prove function can return it?
+    // well-typedness of open_term?
+    let (| e2, c2, d2 |) =
+      check g2 (open_st_term_nv e2 px) pre_e2 (magic ()) (extend_post_hint_opt_g g post_hint g2) in
+
+    if not (stateful_comp c2)
+    then fail g None "Bind: c2 is not st"
+    else
+      let d1 = st_typing_weakening g uvs1 e1 c1 d1 g1 in 
+      // g1 |- ss1 e1 : ss1 c1
+      let d1 = st_typing_subst g1 uvs1 e1 c1 d1 ss1 in
+      let (| e1, c1, d1 |) = add_frame d1 remaining_pre in
+
+      assert (comp_pre c1 == ss1.(comp_pre c10) * remaining_pre);
+      assert (comp_res c1 == ss1.(comp_res c10));
+      assert (None? (lookup g1 x));
+      assert (comp_post c1 == (subst_term (comp_post c10) (shift ss1)) * remaining_pre);
+      assume (open_term remaining_pre x == remaining_pre);
+      assert (open_term (comp_post c1) x == comp_pre c2);
+   
+      let e2_closed = close_st_term e2 x in
+      assume (open_st_term e2_closed x == e2);
+
+      let r = mk_bind' g1 (comp_pre c1) e1 e2_closed c1 c2 px d1 (magic ()) d2 post_hint () in
+
+      k post_hint r
+
+  | _ -> fail g None "Bind: e1 is not an stapp"
+
+// noeq
+// type preamble = {
+//   g0 : env;
+
+//   ctxt : vprop;
+//   ctxt_typing : vprop_typing g0 ctxt;
+
+//   t : st_term;
+//   c : comp_st;
+
+//   uvs : uvs:env { disjoint uvs g0 }
+// }
+
+// let pst_env (#g0:env) (uvs:env { disjoint uvs g0 }) (ss:Psubst.t g0) =
+//   push_env g0 (psubst_env (filter_ss uvs ss) ss)
+
+// noeq
+// type prover_state (preamble:preamble) = {
+//   ss : ss:Psubst.t preamble.g0 {
+//     well_typed_ss preamble.uvs ss
+//   };
+
+//   solved_goals : term;
+
+//   unsolved_goals : list term;
+
+//   remaining_ctxt : list term;
+
+//   steps : st_term;
+
+//   t_typing
+//     : st_typing (pst_env preamble.uvs ss)
+//                 (Psubst.subst_st_term ss preamble.t)
+//                 (Psubst.subst_comp ss preamble.c);
+
+//   unsolved_goals_typing
+//     : vprop_typing (pst_env preamble.uvs ss)
+//                    (list_as_vprop unsolved_goals);
+
+//   remaining_ctxt_typing
+//     : vprop_typing preamble.g0 (list_as_vprop remaining_ctxt);
   
-  steps_typing
-    : st_typing (pst_env preamble.uvs ss)
-                steps
-                (ghost_comp
-                   preamble.ctxt
-                   (tm_star (list_as_vprop remaining_ctxt) solved_goals));
+//   steps_typing
+//     : st_typing (pst_env preamble.uvs ss)
+//                 steps
+//                 (ghost_comp
+//                    preamble.ctxt
+//                    (tm_star (list_as_vprop remaining_ctxt) solved_goals));
 
-  c_pre_inv
-    : vprop_equiv (pst_env preamble.uvs ss)
-                  (Psubst.subst_term ss (comp_pre preamble.c))
-                  (tm_star (list_as_vprop unsolved_goals) solved_goals);
+//   c_pre_inv
+//     : vprop_equiv (pst_env preamble.uvs ss)
+//                   (Psubst.subst_term ss (comp_pre preamble.c))
+//                   (tm_star (list_as_vprop unsolved_goals) solved_goals);
 
-  solved_goals_closed : squash (freevars solved_goals `Set.subset`
-                                dom preamble.g0);
-}
+//   solved_goals_closed : squash (freevars solved_goals `Set.subset`
+//                                 dom preamble.g0);
+// }
 
-let pst_extends (#preamble:_) (p1 p2:prover_state preamble) =
-  p1.ss `Psubst.subst_extends` p2.ss
+// let pst_extends (#preamble:_) (p1 p2:prover_state preamble) =
+//   p1.ss `Psubst.subst_extends` p2.ss
 
-type prover_t =
-  #preamble:_ ->
-  p:prover_state preamble ->
-  T.Tac (option (p':prover_state preamble { p' `pst_extends` p /\
-                                            p'.unsolved_goals == [] }))
+// type prover_t =
+//   #preamble:_ ->
+//   p:prover_state preamble ->
+//   T.Tac (option (p':prover_state preamble { p' `pst_extends` p /\
+//                                             p'.unsolved_goals == [] }))
 
-type prover_step_t =
-  #preamble:_ ->
-  p:prover_state preamble ->
-  prover:prover_t ->
-  T.Tac (option (p':prover_state preamble { p' `pst_extends` p }))
+// type prover_step_t =
+//   #preamble:_ ->
+//   p:prover_state preamble ->
+//   prover:prover_t ->
+//   T.Tac (option (p':prover_state preamble { p' `pst_extends` p }))
 
